benchmark/pigeon_hole.v
@@ -1,0 +1,59 @@
+Require Import List.
+
+Axiom Pigeon_In_Hole : nat -> nat -> Prop.
+
+Definition cons_option {A: Type} (e: option A) (l: list A) :=
+  match e with
+  | None => l
+  | Some v => v:: l
+  end.
+
+Fixpoint map_n (F: nat -> option Prop) (n: nat) :=
+  cons_option (F n)
+              (match n with
+               | O => nil
+               | S n' => map_n F n'
+               end).
+
+Fixpoint or_list (l: list Prop) :=
+  match l with
+  | nil => False
+  | e::nil => e
+  | e::l   => e  \/ or_list l
+  end.
+
+Fixpoint and_list (l: list Prop) :=
+  match l with
+  | nil => True
+  | e::nil => e
+  | e::l   => e /\ and_list l
+  end.
+
+Definition big_or (n:nat) (F: nat -> option Prop)  :=
+  or_list (map_n F n).
+
+Definition big_and (n:nat) (F: nat -> option Prop)  :=
+  and_list (map_n F n).
+
+Fixpoint pigeon_in_hole (b:nat) (n:nat) : Prop :=
+  (big_or n (fun n => Some (Pigeon_In_Hole b n)) /\
+   match b with
+   | O => True
+   | S b' => pigeon_in_hole b' n
+   end).
+
+Fixpoint forall_2 (P : nat -> nat -> option Prop) (i:nat) (j:nat) :=
+  big_and j (P i) /\ match i with
+                     | O => True
+                     | S i' => forall_2 P i' j
+                     end.
+
+Definition at_most_one_pigeon_per_hole (b:nat) (k:nat) :=
+  Some (forall_2 (fun i j => if Nat.ltb i j then  Some (Pigeon_In_Hole i k -> Pigeon_In_Hole j k -> False) else None) b b).
+
+Definition at_most_one_pigeon (b:nat) (n:nat)  :=
+  big_and n (at_most_one_pigeon_per_hole b).
+
+Definition pigeon_hole (b:nat) (n:nat) :=
+  pigeon_in_hole b n /\ at_most_one_pigeon b n.
+
