benchmark/pigeon_itauto.v
@@ -1,0 +1,56 @@
+Require Import Cdcl.Itauto.
+Require Import pigeon_hole.
+
+Goal pigeon_hole 1 0 -> False.
+Proof.
+  unfold pigeon_hole. cbn.
+  Time  vitauto.
+Time Qed.
+
+Goal pigeon_hole 2 1 -> False.
+Proof.
+  unfold pigeon_hole. cbn.
+Time  vitauto.
+Time Qed.
+
+Goal pigeon_hole 3 2 -> False.
+Proof.
+  unfold pigeon_hole. cbn.
+Time  vitauto.
+Time Qed.
+
+Goal pigeon_hole 4 3 -> False.
+Proof.
+  unfold pigeon_hole. cbn.
+Time  vitauto.
+Time Qed.
+
+Goal pigeon_hole 5 4 -> False.
+Proof.
+  unfold pigeon_hole. cbn.
+Time  vitauto.
+Time Qed.
+
+Goal pigeon_hole 6 5 -> False.
+Proof.
+  unfold pigeon_hole. cbn.
+Time  vitauto.
+Time Qed.
+
+Goal pigeon_hole 7 6 -> False.
+Proof.
+  unfold pigeon_hole. cbn.
+Time  vitauto.
+Time Qed.
+
+Goal pigeon_hole 8 7 -> False.
+Proof.
+  unfold pigeon_hole. cbn.
+Time  vitauto.
+Time Qed.
+
+Goal pigeon_hole 9 8 -> False.
+Proof.
+  unfold pigeon_hole. cbn.
+Time  vitauto.
+Time Qed.
